fixup constrainable_update_def, and tweak well_formed_constraints_def
also try to make a start on the new add_constraints_thm

holConstrainedExtensionScript.sml
@@ -6,6 +6,25 @@ val _ = new_theory"holConstrainedExtension"
 
 val mem = ``mem:'U->'U->bool``
 
+(* TODO: move *)
+
+val is_type_valuation_UPDATE_LIST = store_thm("is_type_valuation_UPDATE_LIST",
+  ``∀t ls. is_type_valuation t ∧ EVERY (inhabited o SND) ls ⇒
+           is_type_valuation (t =++ ls)``,
+  rw[is_type_valuation_def,APPLY_UPDATE_LIST_ALOOKUP] >>
+  BasicProvers.CASE_TAC >> rw[] >> imp_res_tac ALOOKUP_MEM >>
+  fs[EVERY_MEM,FORALL_PROD] >> metis_tac[])
+
+val UPDATE_LIST_NOT_MEM = store_thm("UPDATE_LIST_NOT_MEM",
+  ``∀ls f x. ¬MEM x(MAP FST ls) ⇒ (f =++ ls) x = f x``,
+  Induct >> simp[UPDATE_LIST_THM,combinTheory.APPLY_UPDATE_THM])
+
+val MAP_ZIP_UPDATE_LIST_ALL_DISTINCT_same = store_thm("MAP_ZIP_UPDATE_LIST_ALL_DISTINCT_same",
+  ``∀ks vs f. LENGTH ks = LENGTH vs ∧ ALL_DISTINCT ks ⇒ (MAP (f =++ ZIP (ks,vs)) ks = vs)``,
+  Induct >> simp[LENGTH_NIL_SYM] >>
+  gen_tac >> Cases >> simp[UPDATE_LIST_THM] >>
+  simp[UPDATE_LIST_NOT_MEM,MAP_ZIP,combinTheory.APPLY_UPDATE_THM])
+
 val types_in_def = Define`
   types_in (Var x ty) = {ty} ∧
   types_in (Const c ty) = {ty} ∧
@@ -20,20 +39,17 @@ val type_ok_types_in = store_thm("type_ok_types_in",
 
 val constrainable_update_def = Define`
   constrainable_update upd ⇔
-    let axiom_tyvars = set (FLAT (MAP tvars (axioms_of_upd upd))) in
-    let const_tyvars = set (FLAT (MAP (tyvars o SND) (consts_of_upd upd))) in
-    axiom_tyvars = const_tyvars ∧
-    let all_types =
-      BIGUNION (set (MAP types_in (axioms_of_upd upd))) ∪
-      set (MAP SND (consts_of_upd upd)) in
-    ∀name arity args.
-      MEM (name,arity) (types_of_upd upd) ∧
-      Tyapp name args ∈ all_types
-      ⇒
-      (∀args'. Tyapp name args' ∈ all_types ⇒ args' = args) ∧
-      ∃vars. args = MAP Tyvar vars ∧
-             set vars = axiom_tyvars ∧
-             arity = LENGTH args`
+    ∃vars.
+      EVERY ($= (set vars)) (MAP (set o tvars) (axioms_of_upd upd)) ∧
+      EVERY ($= (set vars)) (MAP (set o tyvars o SND) (consts_of_upd upd)) ∧
+      let all_types =
+        BIGUNION (set (MAP types_in (axioms_of_upd upd))) ∪
+        set (MAP SND (consts_of_upd upd)) in
+      ∀name arity args.
+        MEM (name,arity) (types_of_upd upd) ∧
+        Tyapp name args ∈ all_types
+        ⇒
+        args = MAP Tyvar vars ∧ arity = LENGTH args`
 
 val TypeDefn_constrainable = store_thm("TypeDefn_constrainable",
   ``∀name pred abs rep ctxt.
@@ -67,17 +83,17 @@ val TypeDefn_constrainable = store_thm("TypeDefn_constrainable",
     fs[MEM_MAP,EXISTS_PROD] >>
     metis_tac[] ) >>
   simp[constrainable_update_def] >>
+  qexists_tac`STRING_SORT (tvars pred)` >>
+  simp[tyvars_def,Q.SPECL[`set s`,`set t`]EXTENSION,MEM_FOLDR_LIST_UNION,MEM_MAP,PULL_EXISTS,EVERY_MAP] >>
   conj_tac >- (
     simp[conexts_of_upd_def,tvars_def,equation_def,tyvars_def] >>
     simp[EXTENSION,MEM_FOLDR_LIST_UNION,MEM_MAP,PULL_EXISTS,tyvars_def] >>
     rw[EQ_IMP_THM] >> rw[] >>
     imp_res_tac proves_term_ok >> fs[Once has_type_cases] >>
     imp_res_tac WELLTYPED_LEMMA >> fs[tyvars_def] ) >>
+  conj_tac >- metis_tac[] >>
   simp[conexts_of_upd_def,tvars_def,equation_def,tyvars_def] >>
-  rw[] >> fs[] >> rw[] >> fs[] >> TRY(metis_tac[]) >>
-  qexists_tac`STRING_SORT (tvars pred)` >> simp[] >>
-  simp[EXTENSION,MEM_FOLDR_LIST_UNION,MEM_MAP,PULL_EXISTS,tyvars_def] >>
-  rw[EQ_IMP_THM] >> fs[])
+  rw[] >> fs[] >> rw[] >> fs[] >> TRY(metis_tac[]))
 
 val _ = Parse.type_abbrev("constraints",``:'U list -> ('U list # 'U list) option``)
 
@@ -92,21 +108,27 @@ val constrain_interpretation_def = Define`
     (constrain_assignment cs FST (MAP FST (types_of_upd upd)) δ,
      constrain_assignment cs SND (MAP FST (consts_of_upd upd)) γ)`
 
+val _ = Parse.overload_on("tyvars_of_upd",
+  ``λupd. STRING_SORT (tvars (HD (axioms_of_upd upd)))``)
+
 val well_formed_constraints_def = xDefine"well_formed_constraints"`
   well_formed_constraints0 ^mem upd cs δ ⇔
-    ∀vs tyvs tmvs. cs vs = SOME (tyvs,tmvs) ⇒
+    ∀vs tyvs tmvs.
+        cs vs = SOME (tyvs,tmvs) ⇒
+        EVERY inhabited vs ∧
         LENGTH tyvs = LENGTH (types_of_upd upd) ∧
         EVERY inhabited tyvs ∧
-        let vars = STRING_SORT (tvars (HD (axioms_of_upd upd))) in
+        let vars = tyvars_of_upd upd in
         LENGTH vars = LENGTH vs ∧
-        let τ = K boolset =++ (ZIP(vars,vs))in
-        (* TODO: should constrain δ here, or expect it to already be constrained? *)
-        LIST_REL (λv ty. v <: typesem δ τ ty)
-          tmvs (MAP SND (consts_of_upd upd))`
+        ∀τ. is_type_valuation τ ∧ MAP τ vars = vs ⇒
+          (* TODO: should constrain δ here, or expect it to already be constrained? *)
+          LIST_REL (λv ty. v <: typesem δ τ ty)
+            tmvs (MAP SND (consts_of_upd upd))`
 val _ = Parse.overload_on("well_formed_constraints",``well_formed_constraints0 ^mem``)
 
 val constrain_interpretation_equal_on = store_thm("constrain_interpretation_equal_on",
-  ``∀upd cs i ctxt.
+  ``is_set_theory ^mem ⇒
+    ∀upd cs i ctxt.
       well_formed_constraints upd cs (tyaof i) ∧ upd updates ctxt ∧ ctxt extends init_ctxt
       ⇒
       equal_on ctxt i (constrain_interpretation upd cs i)``,
@@ -127,7 +149,273 @@ val constrain_interpretation_equal_on = store_thm("constrain_interpretation_equa
   fs[LET_THM,LIST_REL_EL_EQN] >>
   fs[ZIP_MAP,MEM_MAP,PULL_EXISTS,FORALL_PROD] >>
   imp_res_tac MEM_ZIP_MEM_MAP >> rfs[] >>
-  PairCases_on`p`>>fs[] >> metis_tac[])
+  TRY(PairCases_on`p`>>fs[] >> metis_tac[]) >>
+  first_x_assum(qspec_then`K boolset =++ ZIP(tyvars_of_upd upd,args)`mp_tac) >>
+  discharge_hyps >- (
+    conj_tac >- (
+      match_mp_tac is_type_valuation_UPDATE_LIST >>
+      simp[EVERY_MEM,is_type_valuation_def] >>
+      conj_tac >- metis_tac[setSpecTheory.boolean_in_boolset] >>
+      simp[MEM_ZIP,PULL_EXISTS] >>
+      fs[EVERY_MEM,MEM_EL,PULL_EXISTS]) >>
+    match_mp_tac MAP_ZIP_UPDATE_LIST_ALL_DISTINCT_same >>
+    simp[] ) >>
+  rw[] >> fs[MEM_MAP,EXISTS_PROD] >> metis_tac[])
+
+val valid_constraints_def = xDefine"valid_constraints"`
+  valid_constraints0 ^mem ctxt upd cs i ⇔
+    ∀v.
+      is_valuation (tysof (upd::ctxt))
+        (tyaof (constrain_interpretation upd cs i))
+        v ∧
+      IS_SOME (cs (MAP (tyvof v) (tyvars_of_upd upd)))
+      ⇒
+      ∀p. MEM p (axioms_of_upd upd) ⇒
+        termsem (tmsof (upd::ctxt))
+          (constrain_interpretation upd cs i)
+          v p = True`
+val _ = Parse.overload_on("valid_constraints",``valid_constraints0 ^mem``)
+
+(*
+val add_constraints_thm = store_thm("add_constraints_thm",
+  ``is_set_theory ^mem ⇒
+    ∀i upd ctxt cs.
+      upd updates ctxt ∧ ctxt extends init_ctxt ∧
+      i models (thyof (upd::ctxt)) ∧
+      well_formed_constraints upd cs (tyaof i) ∧
+      valid_constraints ctxt upd cs i
+      ⇒
+      constrain_interpretation upd cs i models thyof (upd::ctxt)``,
+  rw[] >> fs[models_def] >>
+  REWRITE_TAC[CONJ_ASSOC] >>
+  `theory_ok (thyof ctxt)` by metis_tac[extends_theory_ok,init_theory_ok] >>
+  `∃δ γ. i =(δ,γ)` by metis_tac[pair_CASES] >>
+  `ALL_DISTINCT (MAP FST (type_list (upd::ctxt))) ∧
+   ALL_DISTINCT (MAP FST (const_list (upd::ctxt)))` by (
+    conj_tac >>
+    imp_res_tac updates_ALL_DISTINCT >>
+    first_x_assum match_mp_tac >>
+    imp_res_tac extends_ALL_DISTINCT >>
+    first_x_assum match_mp_tac >>
+    EVAL_TAC ) >>
+  conj_asm1_tac >- (
+    fs[is_interpretation_def,is_std_interpretation_def,constrain_interpretation_def] >>
+    simp[GSYM CONJ_ASSOC] >>
+    conj_tac >- (
+      fs[is_type_assignment_def,FEVERY_ALL_FLOOKUP] >> rw[] >>
+      res_tac >> rw[constrain_assignment_def] >>
+      BasicProvers.CASE_TAC >> rw[] >>
+      fs[FLOOKUP_FUNION] >>
+      BasicProvers.CASE_TAC >- metis_tac[] >>
+      fs[well_formed_constraints_def] >>
+      qmatch_assum_rename_tac`cs ls = SOME p`[]>>
+      PairCases_on`p`>>res_tac>>
+      imp_res_tac ALOOKUP_MEM>>
+      rfs[ZIP_MAP,MEM_MAP] >>
+      rfs[EVERY_MEM,MEM_ZIP] >>
+      metis_tac[MEM_EL]) >>
+    CONV_TAC(lift_conjunct_conv(can (match_term ``is_std_type_assignment X``))) >>
+    conj_asm1_tac >- (
+      fs[is_std_type_assignment_def,constrain_assignment_def] >>
+      imp_res_tac theory_ok_sig >>
+      fs[is_std_sig_def,IS_SOME_EXISTS,PULL_EXISTS] >>
+      imp_res_tac ALOOKUP_MEM >>
+      rw[] >> fs[ALL_DISTINCT_APPEND] >>
+      BasicProvers.CASE_TAC >>
+      res_tac >> fs[] >> rw[] >>
+      rpt (BasicProvers.CASE_TAC >> res_tac >> fs[]) >>
+      fs[well_formed_constraints_def] >>
+      qmatch_assum_rename_tac`cs ls = SOME p`["ls"]>>
+      PairCases_on`p`>>res_tac>>
+      imp_res_tac ALOOKUP_MEM >> rfs[MEM_MAP,EXISTS_PROD,ZIP_MAP]>>
+      imp_res_tac MEM_ZIP_MEM_MAP >> rfs[] >>
+      metis_tac[]) >>
+    conj_tac >- (
+      fs[interprets_def,constrain_assignment_def] >> rw[] >>
+      BasicProvers.CASE_TAC >>
+      BasicProvers.CASE_TAC >>
+      imp_res_tac ALOOKUP_MEM >>
+      fs[well_formed_constraints_def] >>
+      qmatch_assum_rename_tac`cs ls = SOME p`["ls"]>>
+      PairCases_on`p`>>res_tac>>
+      fs[LET_THM] >> imp_res_tac LIST_REL_LENGTH >> fs[] >>
+      imp_res_tac MEM_ZIP_MEM_MAP >> rfs[] >>
+      imp_res_tac theory_ok_sig >>
+      fs[is_std_sig_def] >>
+      imp_res_tac ALOOKUP_MEM >>
+      fs[ALL_DISTINCT_APPEND,MEM_MAP,PULL_EXISTS,EXISTS_PROD] >>
+      metis_tac[]) >>
+    fs[is_term_assignment_def,FEVERY_ALL_FLOOKUP] >> rw[] >>
+    first_x_assum(fn th => first_assum(strip_assume_tac o MATCH_MP th)) >>
+    first_x_assum(fn th => first_assum(strip_assume_tac o MATCH_MP th)) >>
+    rw[constrain_assignment_def] >>
+    reverse BasicProvers.CASE_TAC >- (
+      fs[well_formed_constraints_def] >>
+      qmatch_assum_rename_tac`cs ls = SOME p`["ls"]>>
+      PairCases_on`p`>>
+      first_x_assum(fn th => first_assum(strip_assume_tac o MATCH_MP th)) >>
+      fs[LET_THM] >>
+      qpat_assum`FLOOKUP X Y = Z`mp_tac >>
+      simp[FLOOKUP_FUNION] >>
+      BasicProvers.CASE_TAC >- (
+        BasicProvers.CASE_TAC >- (
+          
+        imp_res_tac LIST_REL_LENGTH >> fs[] >> simp[ZIP_MAP] >>
+        BasicProvers.CASE_TAC
+        imp_res_tac ALOOKUP_FAILS >> fs[] >>
+        metis_tac[ALOOKUP_MEM]
+        ) >>
+      rw[] >>
+      `v = ty` by (
+        fs[Once updates_cases] >> rw[] >> fs[] >>
+        qmatch_assum_abbrev_tac`ALOOKUP al k = SOME v` >>
+        `ALL_DISTINCT (MAP FST al)` by (
+          simp[Abbr`al`,MAP_MAP_o,combinTheory.o_DEF,UNCURRY,ETA_AX] ) >>
+        imp_res_tac ALOOKUP_ALL_DISTINCT_MEM >>
+        fs[Abbr`al`] ) >>
+      rw[] >> res_tac >> fs[old_constrain_assignment_def]) >>
+    Cases_on`type_ok (tysof ctxt) v` >- (
+      qmatch_abbrev_tac`a <: b` >>
+      qmatch_assum_abbrev_tac`a <: c` >>
+      qsuff_tac `b = c` >- rw[] >>
+      unabbrev_all_tac >>
+      match_mp_tac typesem_consts >>
+      first_assum(match_exists_tac o concl) >> simp[] >>
+      simp[type_ok_def] >> rw[FUN_EQ_THM] >>
+      BasicProvers.CASE_TAC >>
+      fs[IS_SOME_EXISTS,PULL_EXISTS] >> res_tac >>
+      fs[Once updates_cases] >> rw[] >> fs[] >> rw[] >>
+      imp_res_tac ALOOKUP_MEM >> fs[MEM_MAP,EXISTS_PROD] >>
+      metis_tac[] ) >>
+    qpat_assum`FLOOKUP X Y = Z`mp_tac >>
+    simp[FLOOKUP_FUNION] >>
+    BasicProvers.CASE_TAC >- (
+      strip_tac >>
+      fs[theory_ok_def] >>
+      qsuff_tac`F`>-rw[]>>
+      qpat_assum`¬x`mp_tac >>simp[]>>
+      first_x_assum match_mp_tac >>
+      simp[IN_FRANGE_FLOOKUP] >>
+      metis_tac[] ) >>
+    rw[] >>
+    qmatch_abbrev_tac`a <: b` >>
+    qmatch_assum_abbrev_tac`a <: c` >>
+    qsuff_tac `b = c` >- rw[] >>
+    unabbrev_all_tac >>
+    fs[Once updates_cases] >> rw[] >> fs[] >- (
+      rpt AP_THM_TAC >> AP_TERM_TAC >> rw[FUN_EQ_THM] ) >>
+    qmatch_abbrev_tac`typesem d1 τ v = typesem δ τ v` >>
+    `is_std_type_assignment d1 ∧
+     is_std_type_assignment δ` by (
+       reverse conj_asm2_tac >- fs[is_std_interpretation_def] >>
+       simp[Abbr`d1`,GSYM old_constrain_assignment_def] ) >>
+    rator_x_assum`ALOOKUP` mp_tac >> simp[] >>
+    Q.PAT_ABBREV_TAC`t1 = domain (typeof pred)` >>
+    Q.PAT_ABBREV_TAC`t2 = Tyapp name X` >>
+    qsuff_tac`k ∈ {abs;rep} ∧ (set (tyvars v) = set (tyvars (Fun t1 t2))) ⇒
+              (typesem d1 τ t1 = typesem δ τ t1) ∧
+              (typesem d1 τ t2 = typesem δ τ t2)` >- (
+      match_mp_tac SWAP_IMP >> strip_tac >>
+      discharge_hyps >- (
+        pop_assum mp_tac >> rw[] >>
+        simp[tyvars_def] >>
+        metis_tac[pred_setTheory.UNION_COMM] ) >>
+      pop_assum mp_tac >>
+      rw[] >>
+      qmatch_abbrev_tac`typesem d1 τ (Fun dom rng) = typesem δ τ (Fun dom rng)` >>
+      qspecl_then[`δ`,`τ`,`dom`,`rng`]mp_tac typesem_Fun >>
+      qspecl_then[`d1`,`τ`,`dom`,`rng`]mp_tac typesem_Fun >>
+      simp[] >> rw[]) >>
+    strip_tac >>
+    conj_tac >- (
+      unabbrev_all_tac >>
+      match_mp_tac typesem_consts >>
+      qexists_tac`tysof (ctxt)` >>
+      imp_res_tac proves_term_ok >>
+      qpat_assum`k ∈ X`kall_tac >>
+      fs[term_ok_def] >>
+      conj_tac >- (
+        imp_res_tac term_ok_type_ok >>
+        fs[theory_ok_def] ) >>
+      simp[type_ok_def] >> rw[FUN_EQ_THM] >>
+      BasicProvers.CASE_TAC >>
+      fs[IS_SOME_EXISTS,PULL_EXISTS] >> res_tac >>
+      imp_res_tac ALOOKUP_MEM >>
+      fs[MEM_MAP,EXISTS_PROD] >> metis_tac[] ) >>
+    unabbrev_all_tac >>
+    simp[typesem_def,MAP_MAP_o,combinTheory.o_DEF,ETA_AX] >>
+    BasicProvers.CASE_TAC >>
+    qsuff_tac`set (tyvars v) = set (tvars pred)` >- (
+      qpat_assum`set (tyvars v) = X`kall_tac >>
+      rw[] >>
+      `STRING_SORT (tvars pred) = STRING_SORT (tyvars v)` by (
+        `ALL_DISTINCT (tvars pred)` by simp[] >>
+        `ALL_DISTINCT (tyvars v)` by simp[] >>
+        `PERM (tvars pred) (tyvars v)` by (
+          match_mp_tac sortingTheory.PERM_ALL_DISTINCT >>
+          fs[pred_setTheory.EXTENSION] ) >>
+        metis_tac[holSyntaxLibTheory.STRING_SORT_EQ] ) >>
+      fs[IS_SOME_EXISTS,PULL_EXISTS,LET_THM] >>
+      metis_tac[optionTheory.NOT_SOME_NONE] ) >>
+    simp[tyvars_def,pred_setTheory.EXTENSION,
+         holSyntaxLibTheory.MEM_FOLDR_LIST_UNION,
+         MEM_MAP,PULL_EXISTS] >>
+    qpat_assum`k ∈ X`kall_tac >>
+    imp_res_tac proves_term_ok >> fs[term_ok_def] >>
+    fs[WELLTYPED] >>
+    imp_res_tac tyvars_typeof_subset_tvars >>
+    fs[pred_setTheory.SUBSET_DEF,tyvars_def] >>
+    metis_tac[] ) >>
+  gen_tac >>
+  qmatch_abbrev_tac`P ⇒ q` >>
+  strip_tac >> qunabbrev_tac`q` >>
+  first_x_assum(qspec_then`p`mp_tac) >>
+  fs[Abbr`P`] >>
+  disch_then kall_tac >>
+  first_x_assum(qspec_then`p`mp_tac) >> simp[] >>
+  strip_tac >>
+  `term_ok (sigof ctxt) p` by fs[theory_ok_def] >>
+  imp_res_tac theory_ok_sig >>
+  match_mp_tac satisfies_extend >>
+  map_every qexists_tac[`tysof ctxt`,`tmsof ctxt`] >>
+  simp[] >>
+  REWRITE_TAC[CONJ_ASSOC] >>
+  conj_asm1_tac >- (
+    conj_tac >>
+    match_mp_tac SUBMAP_FUNION >>
+    disj2_tac >>
+    fs[ALL_DISTINCT_APPEND,pred_setTheory.IN_DISJOINT] >>
+    metis_tac[] ) >>
+  match_mp_tac satisfies_consts >>
+  qexists_tac`i` >> simp[] >> fs[] >>
+  simp[term_ok_def,type_ok_def] >>
+  REWRITE_TAC[CONJ_ASSOC] >>
+  conj_tac >- (
+    rw[old_constrain_interpretation_def,old_constrain_assignment_def,FUN_EQ_THM] >>
+    BasicProvers.CASE_TAC >>
+    fs[IS_SOME_EXISTS,PULL_EXISTS] >> res_tac >>
+    fs[ALL_DISTINCT_APPEND,MEM_MAP,EXISTS_PROD] >>
+    imp_res_tac ALOOKUP_MEM >>
+    metis_tac[] ) >>
+  fs[satisfies_def] >> rw[] >>
+  qmatch_assum_abbrev_tac`tmsof ctxt ⊑ tmsig` >>
+  qmatch_assum_abbrev_tac`tysof ctxt ⊑ tysig` >>
+  first_assum(
+    mp_tac o MATCH_MP(REWRITE_RULE[GSYM AND_IMP_INTRO](UNDISCH extend_valuation_exists))) >>
+  first_assum(fn th => disch_then (mp_tac o C MATCH_MP th)) >>
+  discharge_hyps >- fs[is_interpretation_def] >> strip_tac >>
+  first_x_assum(qspec_then`v'`mp_tac) >> simp[] >>
+  disch_then (SUBST1_TAC o SYM) >>
+  match_mp_tac EQ_TRANS >>
+  qexists_tac`termsem (tmsof ctxt) (δ,γ) v' p` >>
+  conj_tac >- (
+    match_mp_tac termsem_frees >>
+    simp[] >> rw[] >>
+    first_x_assum match_mp_tac >>
+    imp_res_tac term_ok_VFREE_IN >>
+    fs[term_ok_def] ) >>
+  metis_tac[termsem_extend])
+*)
 
 val old_constrain_assignment_def = Define`
   old_constrain_assignment cs f =
